Program-proofs/Exercises/2D-counting/prob06/prob06.dfy
@@ -4,24 +4,17 @@
    This is exercise 9.7 from the PC reader
 */
 
-ghost predicate IncrDesc(f:(nat,nat) -> int) 
-{
-    // Expresses the property that f is increasing in its first  
-    // argument and descending in its second argument, i.e. 
-    // ∀ i,j,k ∈ ℕ:
-    //   if i < j then f(i,k) < f(j,k)
-    //   if j ≤ k then f(i,j) ≥ f(i,k)
-  (forall i,j,k:: i <  j  ==>  f(i,k) <  f(j,k)) &&
-  (forall i,j,k:: j <= k  ==>  f(i,j) >= f(i,k))
-}
+include "../../commonSupport.dfy"
+import opened MonotonicityProps
+import opened CommonFunctions
 
 method problem06(g:(nat,nat) -> int, n:nat, w:int) 
 returns (z: int)
-requires IncrDesc(g)
-ensures z == ???
+requires Ordered2DNat(g, Incr, Desc)
+ensures z == ??? 
 {
   /* 
-    Given is a function g: ℕ × ℕ → ℤ that is ascending in 
+    Given is a function g: ℕ × ℕ → ℤ that is increasing in 
     its first argument and descending in its second argument.
 
     Derive a command sequence T that satisfies the following 
@@ -31,12 +24,13 @@ ensures z == ???
       const w : ℤ;
       var   z : ℤ;
       
-        {P : Z = #{ (i,j) | i,j: 0 ≤ i < n ∧ 0 ≤ j < n ∧ i + j < n ∧ g(i,j) = w } }
+        {P : Z = #{ (i,j) | i,j: 0 ≤ i < n ∧ 0 ≤ j < n 
+                                 ∧ i + j < n ∧ g(i,j) = w } }
       T
         {Q : Z = z}
       
-    Note that Z (uppercase) is a specification constant, not a program variable, 
-    whereas z (lowercase) is a program variable. 
+    Note that Z (uppercase) is a specification constant, not a
+    program variable, whereas z (lowercase) is a program variable. 
     The time complexity of T should be in O(n).
   */
 }
